ITree_Deadlock.thy
@@ -7,10 +7,10 @@ begin
 text \<open> Deadlock is an interaction with no visible event \<close>
 
 definition deadlock :: "('e, 'r) itree" where
-"deadlock = Vis [\<mapsto>]"
+"deadlock = Vis {\<mapsto>}"
 
 lemma deadlock_trace_to: "deadlock \<midarrow>tr\<leadsto> P \<longleftrightarrow> tr = [] \<and> P = deadlock"
-  by (metis deadlock_def domIff trace_to_Nil trace_to_VisE)
+  by (auto simp add: deadlock_def)
 
 definition deadlock_free :: "('e, 'r) itree \<Rightarrow> bool" where
 "deadlock_free P = (\<forall> tr. \<not> P \<midarrow>tr\<leadsto> deadlock)"
